% Appendix B File

\refstepcounter{chapter}%
\chapter*{\thechapter \quad Mathematical Background}
\label{appendixB}

\section{Change of Variables in N Dimensions} \label{COV}

In this Subsection we will follow \cite{risken1996fokker}. Let $\bm{x}\in\R^n$ and $t\in[t_0,t_1]$ and the system
\begin{equation}
\begin{cases}
\left(\frac{\partial V}{\partial t}+\sum\limits^{n}_{i=1}a_i\frac{\partial V}{\partial x_i}+\sum\limits^{n}_{i,j=1}b_{ij}\frac{\partial^2V}{\partial x_i\partial x_j}\right)(t,\bm{x})=0\\
V(t_1,\bm{x})=g(\bm{x}).
\end{cases}
\label{Kolmogorov_Backward_Equation_MD}
\end{equation}
We want to see how (\ref{Kolmogorov_Backward_Equation_MD}) changes when we introduce a new system of coordinates in the space $\bm{y}=(y_1,\dots,y_n)^T$ with $y_i=f(\bm{x})$. We are going to analyze the particular case where the change of coordinates is an injective transformation of each one of the spatial dimensions, i.e. $y_i=f(\bm{x})=f(x_i)$. Then if $v(t,\bm{y}(\bm{x}))=V(t,\bm{x})$ is a solution of (\ref{Kolmogorov_Backward_Equation_MD}), it is also a solution of
\begin{equation}
\begin{cases}
\frac{\partial v}{\partial t}+\sum\limits^{n}_{i=1}\underbrace{\frac{\partial y_i}{\partial x_i}a_i(t,\bm{x})}_{a^*_i(t,\bm{y})}\frac{\partial v}{\partial y_i}+\sum\limits^{n}_{i,j=1}\underbrace{\frac{\partial y_j}{\partial x_j}\frac{\partial y_i}{\partial x_i}b_{ij}(t,\bm{x})}_{b^*_{ij}(t,\bm{y})}\frac{\partial^2v}{\partial y_i\partial y_j}=0\\
v(t_1,\bm{y})=V(t_1,f^{-1}(\bm{y}))=g(f^{-1}(\bm{y}))=g^*(\bm{y})\\
\bm{x}=f^{-1}(\bm{y}).
\end{cases}
\end{equation}
Then we have that $v(t,\bm{y})$ is the solution of
\begin{equation}
\begin{cases}
\left(\frac{\partial v}{\partial t}+\sum\limits^{n}_{i=1}a^*_i\frac{\partial v}{\partial y_i}+\sum\limits^{n}_{i,j=1}b^*_{ij}\frac{\partial^2v}{\partial y_i\partial y_j}\right)(t,\bm{y})=0\\
v(t_1,\bm{y})=g^*(\bm{y}),
\end{cases}
\end{equation}
where we have used
\begin{equation}
\frac{\partial v}{\partial x_i}=\frac{\partial v}{\partial y_i}\frac{\partial y_i}{\partial x_i},\quad\frac{\partial^2v}{\partial x_i\partial x_j}=\frac{\partial^2v}{\partial y_i\partial y_j}\frac{\partial y_j}{\partial x_j}\frac{\partial y_i}{\partial x_i}.
\end{equation}

% Copyright 2010 Imran Shafique Ansari
% Contact Email: imran.ansari@kaust.edu.sa
% Contact Number: +966 59 897 1005
